\begin{mitframe}{014-3}

    \mdfsubtitle{Legendre Transforms (Box 14-3)} 
    
\begin{listone}
        
    \item $y^{(k)}=y^{(\init)}-\sum\limits_{\state=1}^{k}\conjcoortwo_{\state}\mathrm{d}\conjcoor$
    
    %benjie: not sure about y^{(k)}
        
	\item $\mathrm{d}y^{(k)}=-\sum\limits_{\state=1}^{k}\conjcoor\mathrm{d}\conjcoortwo_{\state}+\sum\limits_{\state=k+1}^{m}\conjcoortwo_{\state}\mathrm{d}\conjcoor$ 
         
    %benjie: not sure if 'm' , also with 'k'    
         
	\item $\bigg(\dfrac{\partial y^{(k)}}{\partial\conjcoortwo_{\state}}\bigg)_{\conjcoortwo_{\state},...,[\conjcoortwo_{\state}],x_{k+1},...,x_{m}}=-\conjcoor$
    
	\item $\bigg(\dfrac{\partial y^{(k)}}{\partial\conjcoor}\bigg)_{\conjcoortwo_{\state},...,\conjcoortwo_{k},x_{k+1},...,[x_{\state}],...,x_{m}}=\conjcoortwo_{\state}$
        
\end{listone}			

\end{mitframe}